Add user facing bits of the difference

src/Std/Data/DTreeMap/Basic.lean
@@ -1050,7 +1050,7 @@ Computes the difference of the given tree maps.
 This function always iterates through the smaller map.
 -/
 def diff (t₁ t₂ : DTreeMap α β cmp) : DTreeMap α β cmp :=
-    letI : Ord α := ⟨cmp⟩; ⟨t₁.inner.diff t₂.inner t₁.wf.balanced, @Impl.WF.diff α β _ t₁.inner t₁.wf t₂.inner t₂.wf⟩
+    letI : Ord α := ⟨cmp⟩; ⟨t₁.inner.diff t₂.inner t₁.wf.balanced, @Impl.WF.diff α β _ t₁.inner t₁.wf t₂.inner⟩
 
 instance : SDiff (DTreeMap α β cmp) := ⟨diff⟩
 
