src/Std/Data/DTreeMap/Internal/Lemmas.lean
@@ -47,7 +47,7 @@ macro_rules
     | apply WF.constInsertMany | apply WF.constInsertManyIfNewUnit
     | apply WF.alter | apply WF.constAlter
     | apply WF.modify | apply WF.constModify
-    | apply WF.filterMap | apply WF.filter | apply WF.map | apply WF.union) <;> wf_trivial)
+    | apply WF.filterMap | apply WF.filter | apply WF.map | apply WF.union | apply WF.diff) <;> wf_trivial)
 
 /-- Internal implementation detail of the tree map -/
 scoped macro "empty" : tactic => `(tactic| { intros; simp_all [List.isEmpty_iff] } )
@@ -67,6 +67,7 @@ private meta def modifyMap : Std.HashMap Name Name :=
     [⟨`insert, ``toListModel_insert⟩,
      ⟨`insertIfNew, ``toListModel_insertIfNew⟩,
      ⟨`union, ``toListModel_union_list⟩,
+     ⟨`diff, ``toListModel_diff_list⟩,
      ⟨`erase, ``toListModel_erase⟩,
      (`insertMany, ``toListModel_insertMany_list),
      (`Const.insertMany, ``Const.toListModel_insertMany_list),
