src/Std/Data/DTreeMap/Internal/WF/Lemmas.lean
@@ -1632,6 +1632,10 @@ theorem WF.eraseMany! {_ : Ord α} [TransOrd α] {ρ} [ForIn Id ρ α] {l : ρ}
     {t : Impl α β} (h : t.WF) : (t.eraseMany! l).1.WF :=
   (t.eraseMany! l).2 h (fun _ _ h' => h'.erase!)
 
+/-!
+### `eraseManyEntries`
+-/
+
 theorem eraseManyEntries!_eq_foldl {_ : Ord α} {l : List ((a : α) × β a)} {t : Impl α β} :
     (t.eraseManyEntries! l).val = l.foldl (init := t) fun acc ⟨k, _⟩ => acc.erase! k := by
   simp [eraseManyEntries!, ← List.foldl_hom Subtype.val, List.forIn_pure_yield_eq_foldl]
@@ -1693,9 +1697,6 @@ theorem toListModel_eraseManyEntries!_impl {_ : Ord α} [BEq α] [LawfulBEqOrd �
   rw [← eraseManyEntries_eq_eraseManyEntries!_impl h₁.balanced]
   apply toListModel_eraseManyEntries_impl h₁
 
-/-!
-### `eraseMany!`
--/
 
 theorem WF.eraseManyEntries! {_ : Ord α} [TransOrd α] {ρ} [ForIn Id ρ ((a : α) × β a)] {l : ρ}
     {t : Impl α β} (h : t.WF) : (t.eraseManyEntries! l).1.WF :=
@@ -2063,6 +2064,39 @@ theorem WF.filter! {_ : Ord α} {t : Impl α β} {f : (a : α) → β a → Bool
     (t.filter! f).WF := by
   rw [← filter_eq_filter! (h := h.balanced)]
   exact h.filter
+
+/-!
+### diff
+-/
+
+theorem toListModel_diff_list {_ : Ord α} [BEq α] [LawfulBEqOrd α] [TransOrd α]
+    {t₁ t₂ : Impl α β} (h₁ : t₁.WF) (h₂ : t₂.WF) :
+    List.Perm (t₁.diff t₂ h₁.balanced).toListModel (t₁.toListModel.filter (fun p => !containsKey p.fst t₂.toListModel)) := by
+  rw [diff]
+  split
+  · simp only [toListModel_filter]
+    conv =>
+      lhs
+      lhs
+      ext e
+      congr
+      rw [contains_eq_containsKey h₂.ordered]
+  · apply toListModel_eraseManyEntries_impl h₁
+
+theorem diff_eq_diff! [Ord α]
+    {t₁ t₂ : Impl α β} (h₁ : t₁.WF) :
+    (t₁.diff t₂ h₁.balanced) = t₁.diff! t₂ := by
+  simp only [diff, diff!]
+  split
+  · rw [filter_eq_filter!]
+  . rw [eraseManyEntries_eq_eraseManyEntries!_impl h₁.balanced]
+
+theorem WF.diff! {_ : Ord α} [TransOrd α]
+    {t₁ : Impl α β} (h₁ : t₁.WF) {t₂ : Impl α β} : (t₁.diff! t₂).WF := by
+  simp only [Impl.diff!]
+  split
+  . exact WF.filter! h₁
+  . exact WF.eraseManyEntries! h₁
 
 /-!
 ### map
